deprecate Vector.empty

Batteries/Data/Vector/Basic.lean
@@ -35,6 +35,10 @@ namespace Vector
 
 @[deprecated (since := "2024-11-20")] alias eraseIdxN := eraseIdx
 
+/-- Use `#v[]` instead. -/
+@[deprecated "Use `#v[]`." (since := "2024-11-27")]
+def empty (α : Type u) : Vector α 0 := #v[]
+
 /--
 Returns `true` when all elements of the vector are pairwise distinct using `==` for comparison.
 -/
